proof/security/PKE_Ext.ec
@@ -1,9 +1,168 @@
-require import PROM.
-require PKE.
+require import AllCore List Distr DBool PROM_Ext.
 
-clone include PKE.
+require LorR. 
+clone import LorR as LorR' with
+  type input <- unit.  
 
-(* Fix me. Move to Library. *)
+type pkey.
+type skey.
+type plaintext.
+type ciphertext.
+
+module type Scheme = {
+  proc kg() : pkey * skey
+  proc enc(pk:pkey, m:plaintext)  : ciphertext
+  proc dec(sk:skey, c:ciphertext) : plaintext option
+}.
+
+module type Adversary = {
+  proc choose(pk:pkey)     : plaintext * plaintext
+  proc guess(c:ciphertext) : bool
+}.
+
+module CPA (S:Scheme, A:Adversary) = {
+  proc main() : bool = {
+    var pk : pkey;
+    var sk : skey;
+    var m0, m1 : plaintext;
+    var c : ciphertext;
+    var b, b' : bool;
+
+    (pk, sk) <@ S.kg();
+    (m0, m1) <@ A.choose(pk);
+    b        <$ {0,1};
+    c        <@ S.enc(pk, b ? m1 : m0);
+    b'       <@ A.guess(c);
+    return (b' = b);
+  }
+}.
+
+module CPA_L (S:Scheme, A:Adversary) = {
+  proc main() : bool = {
+    var pk : pkey;
+    var sk : skey;
+    var m0, m1 : plaintext;
+    var c : ciphertext;
+    var b' : bool;
+
+    (pk, sk) <@ S.kg();
+    (m0, m1) <@ A.choose(pk);
+    c        <@ S.enc(pk, m0);
+    b'       <@ A.guess(c);
+    return b';
+  }
+}.
+
+module CPA_R (S:Scheme, A:Adversary) = {
+  proc main() : bool = {
+    var pk : pkey;
+    var sk : skey;
+    var m0, m1 : plaintext;
+    var c : ciphertext;
+    var b' : bool;
+
+    (pk, sk) <@ S.kg();
+    (m0, m1) <@ A.choose(pk);
+    c        <@ S.enc(pk, m1);
+    b'       <@ A.guess(c);
+    return b';
+  }
+}.
+
+section.
+
+  declare module S <: Scheme.
+  declare module A <: Adversary{-S}.
+
+  lemma pr_CPA_LR &m: 
+    islossless S.kg => islossless S.enc =>
+    islossless A.choose => islossless A.guess => 
+    `| Pr[CPA_L(S,A).main () @ &m : res] - Pr[CPA_R(S,A).main () @ &m : res] | =
+     2%r * `| Pr[CPA(S,A).main() @ &m : res] - 1%r/2%r |.
+  proof.
+    move => kg_ll enc_ll choose_ll guess_ll.
+    have -> : Pr[CPA(S, A).main() @ &m : res] = 
+              Pr[RandomLR(CPA_R(S,A), CPA_L(S,A)).main() @ &m : res].
+    + byequiv (_ : ={glob S, glob A} ==> ={res})=> //.
+      proc.      
+      swap{1} 3-2; seq 1 1 : (={glob S, glob A, b}); first by rnd.
+      if{2}; inline *; wp; do 4! call (_: true); auto => /> /#.
+    rewrite -(pr_AdvLR_AdvRndLR (CPA_R(S,A)) (CPA_L(S,A)) &m) 2:/#.
+    byphoare => //; proc.
+    by call guess_ll; call enc_ll; call choose_ll; call kg_ll.
+  qed.
+
+end section.
+
+(*
+** Based on lists. Several versions can be given as in RandOrcl.
+** Also, oracle annotations could be used to provide different oracles during
+** the choose and guess stages of the experiment.
+*)
+const qD : int.
+
+axiom qD_pos : 0 < qD.
+
+module type CCA_ORC = {
+  proc dec(c:ciphertext) : plaintext option
+}.
+
+module type CCA_ADV (O:CCA_ORC) = {
+  proc choose(pk:pkey)     : plaintext * plaintext {O.dec}
+  proc guess(c:ciphertext) : bool {O.dec}
+}.
+
+module CCA (S:Scheme, A:CCA_ADV) = {
+  var log : ciphertext list
+  var cstar : ciphertext option
+  var sk : skey
+
+  module O = {
+    proc dec(c:ciphertext) : plaintext option = {
+      var m : plaintext option;
+
+      if (size log < qD && (Some c <> cstar)) {
+        log <- c :: log;
+        m   <@ S.dec(sk, c);
+      }
+      else m <- None;
+      return m;
+    }
+  }
+
+  module A = A(O)
+
+  proc main() : bool = {
+    var pk : pkey;
+    var m0, m1 : plaintext;
+    var c : ciphertext;
+    var b, b' : bool;
+
+    log      <- [];
+    cstar    <- None;
+    (pk, sk) <@ S.kg();
+    (m0, m1) <@ A.choose(pk);
+    b        <$ {0,1};
+    c        <@ S.enc(pk, b ? m1 : m0);
+    cstar    <- Some c;
+    b'       <@ A.guess(c);
+    return (b' = b);
+  }
+}.
+
+module Correctness (S:Scheme) = {
+  proc main(m:plaintext) : bool = {
+    var pk : pkey;
+    var sk : skey;
+    var c  : ciphertext;
+    var m' : plaintext option;
+
+    (pk, sk) <@ S.kg();
+    c        <@ S.enc(pk, m);
+    m'       <@ S.dec(sk, c);
+    return (m' = Some m);
+  }
+}.
 
 module type CAdversary = {
    proc find(pk : pkey, sk : skey) : plaintext 
@@ -25,25 +184,16 @@ module CorrectnessAdv(S : Scheme, A : CAdversary) = {
 
 clone import FullRO as RO.
 
-module type RO_ti = {
-  proc init() : unit
-  proc h(_: in_t) : out_t
-}.
-
-module type RO_t = {
-  include RO_ti [h]
-}.
-
-module type SchemeRO(H : RO_t) = {
+module type SchemeRO(H : ROpub) = {
   include Scheme
 }.
 
 
-module type AdversaryRO(H : RO_t) = {
+module type AdversaryRO(H : ROpub) = {
   include Adversary
 }.
 
-module type CAdversaryRO(H : RO_t) = {
+module type CAdversaryRO(H : ROpub) = {
   include CAdversary
 }.
 
@@ -51,10 +201,11 @@ module type CPAGame(S: Scheme, A : Adversary) = {
    proc main() : bool
 }.
 
-module CPAGameROM(G : CPAGame, S : SchemeRO, A : AdversaryRO, H : RO_ti) = {
+module CPAGameROM(G : CPAGame, S : SchemeRO, A : AdversaryRO, O : RO) = {
+   module H = Pub(O)
    proc main() : bool = {
      var b;
-     H.init();
+     O.init();
      b <@ G(S(H),A(H)).main();
      return b;
    }
@@ -68,10 +219,11 @@ module type CGame(S: Scheme, A : CAdversary) = {
    proc main() : bool
 }.
 
-module CGameROM(G : CGame, S : SchemeRO, A : CAdversaryRO, H : RO_ti) = {
+module CGameROM(G : CGame, S : SchemeRO, A : CAdversaryRO, O : RO) = {
+   module H = Pub(O)
    proc main() : bool = {
      var b;
-     H.init();
+     O.init();
      b <@ G(S(H),A(H)).main();
      return b;
    }
